# Lecture 13

## Example of `value-of` a `diff-exp`
```scheme
(value-of <<-(-(x,3), -(v,i))>> p) =
    (-
      (-
        (value-of <<x>> p)
          (value-of <<3>> p))
      (value-of <<-(v,i)>> p))
```

## Behavior of a Program
> (value-of-program ~~exp~~ prg) = ?

```scheme
Program     ::== Expression
                 a-program (exp1)
Expression  ::== Number
                 const-exp (num)
Expression  ::== -(Expression , Expression)
                 diff-exp (exp1 exp2)
Expression  ::== zero? (Expression)
                 zero?-exp (exp1)
Expression  ::== if Expression then Expression else Expression
                 if-exp (exp1 exp2 exp3)
Expression  ::== Identifier
                 var-exp (var)
Expression  ::== let Identifier = Expression in Expression
                 let-exp (var exp1 body) ;'body' being the scope
```

> (value-of-program ~~exp~~ prg) = `(value-of prg p)`

## `value-of` a `zero?-exp`
```
Exporession ::== zero? (Expression)
                 zero?-exp (exp1)
```

Steps:
1. Evaluate exp1
2. Compare x with 0
3. if x == 0, return true
4. else false

### Inference Rules
```
        (value-of exp1 p) = val1
----------------------------------------
(value-of (zero?-exp exp1) p)
  =  { (bool-val #t)    if (expval->num val1) = 0 }
     { (bool-val #f)    if (expval->num val1) != 0 }
```

## `value-of` an `if-exp`
```
Expression ::== if Expression then Expression else Expression
                if-exp (exp1 exp2 exp3)
```

Steps:
1. Evaluate exp1 (call it, idk, val1?)
2. If val1, evaluate exp2
3. If !val1, evaluate exp3

### Inference Rules
```
        (value-of exp1 p) = val1
----------------------------------------
(value-of (if-exp exp1 exp2 exp3) p)
  =  { (value-of exp2 p)    if(expval->bool val1) = #t }
     { (value-of exp3 p)    if(expval->bool val1) = #f }
```

# KNOW HOW TO WRITE INFERENCE RULES!!!
"You might need to write something like this on an exam...."

## Example Scheme Code...

> (value-of (if-exp exp1 exp2 exp3) p) = 

```scheme
(if(expval->bool (value-of exp1 p))
  (value-of exp2 p)     ;then branch
  (value-of exp3 p))    ;else branch
```

## An Example With Values
Assume p = [x=33,y=22]

```scheme
(value-of <<if zero?(-(x,11)) then -(y,2) else (y,4)>> p)
```
> This subtracts 4 from `y`. AKA exp3 gets evaluated.

And here's how it would be executed in actual code:
```scheme
(if (expval->bool (value-of <<zero?(-(x,11))>> p))
    (value-of <<-(y,2)>> p)
    (value-of <<-(y,4)>> p))
```

Here we go....

## `value-of` a `let-exp`
"Defining local variables in some scope."

### Let example 1
```
let x = 5
    in -(x,3)
```
> Output: 2

"I know it's trivial, but I'm gonna say it. A let expression evaluates to the value of its body. Whatever comes after `in`, is the body of the `let`."

### Let example 2
```scheme
let z = 5                       ;z = 5
    in let x = 3                ;x = 3
        in let y = -(x,1)       ;y = 2, x = 3
            in let x = 4        ;x = 4
                in -(z, -(x,y)) ;x = 4, y = 2, z = 5
```
> This just evaluates to 3.


## `value-of` a `let-exp` (finally lol)
```
        (value-of exp1 p) = val1
----------------------------------------
(value-of (let-exp var exp1 body) p)
   = (value-of body [var=val1]p)
```

Scheme:
`(value-of (let-exp var exp1 body) œÅ) =`
```scheme
(value-of body [var=(value-of exp1 p)]p)
```

## An Example Written in Code:
```scheme
(value-of
    <<let x = 7
      in let y = 2
        in let y = let x = -(x,1) in -(x,y)
          in -(-(x,8),y)>>
p0)
```